\documentclass{article}
\usepackage[margin=1in]{geometry}
\usepackage{amsmath}
\usepackage{amssymb}
\usepackage{amsthm}
\usepackage{graphicx}
\graphicspath{images/}

\begin{document}

\title{MC Estimation of a Downward Closed Set of Subsets}
\author{Aresh Pourkavoos}
\maketitle

\newcommand{\E}{\mathbb{E}}
\newcommand{\abs}[1]{\left\vert #1 \right\vert}
\newcommand{\norm}[1]{\left\Vert #1 \right\Vert}

$V = \{v_1, \ldots, v_n\}$ finite set, $T$ predicate on subsets of $V$ \\
$A \subseteq B, T(B) \rightarrow T(A)$ ($T$ downward closed) \\
Notation:
\begin{itemize}
\item
  $\binom{V}{k} := \{B \subseteq V | \abs{B} = k\}$
\item
  $S_n := $ set of permutations on $\{1, \ldots, n\}$
\item
  $V_{\pi(:k)} := \left\{v_{\pi(i)} \middle| 1 \leq i \leq k\right\}$ for $\pi \in S_n$
\item
  $[T(B)]$ is the Iverson bracket: $1$ if $T(B)$ is true, $0$ otherwise
\item
  Expectations over e.g. $\pi \in S_n$ are uniform
\end{itemize}
Want to estimate
\begin{align*}
  &\abs{\left\{B \subseteq V \middle| T(B)\right\}} \\
  =\ &\sum_{k=0}^n\abs{\left\{B \in \binom{V}{k} \middle| T(B)\right\}} \\
  =\ &\sum_{k=0}^n\binom{n}{k}\E_{B \in \binom{V}{k}}([T(B)]) \\
  =\ &\sum_{k=0}^n\binom{n}{k}\E_{\pi \in S_n}\left(\left[T\left(V_{\pi(:k)}\right)\right]\right) \\
  =\ &\E_{\pi \in S_n}\left(\sum_{k=0}^n\binom{n}{k}\left[T\left(V_{\pi(:k)}\right)\right]\right) \\
\end{align*}
Simple MC method: sample random permutation of $V$, add $\binom{n}{k}$ for each $V_{\pi(:k)}$ satisfying $T$ \\
Since $T$ downward closed, first (smallest) value of $k$ such that $\lnot T(V_{\pi(:k)})$ makes all subsequent terms $0$: formalized later \\
Next, WTS this is equivalent to choosing new elements of the permutation ``on the fly'' \\
Define $x_B$ to be the expected sum remaining after $B \subseteq V$ has already been chosen as the prefix: \\
\[
x_B :=
\begin{cases}
  0 & \text{if $\lnot T(B)$} \\
  1 & \text{if $T(B)$ and $B = V$} \\
  \binom{n}{\abs{B}}+\E_{v \in V \setminus B}\left(x_{B \cup \{v\}}\right) & \text{if $T(B)$ and $B \neq V$}
\end{cases}
\]
\newtheorem{lemma}{Lemma}
\newtheorem{theorem}{Theorem}
\begin{lemma}
  For all $B \subseteq V$, $x_B = \E_{\pi \in S_n}\left(\sum_{k=\abs{B}}^n\binom{n}{k}\left[T\left(V_{\pi(:k)}\right)\right] \middle| B = V_{\pi(:\abs{B})}\right)$.
\end{lemma}
\begin{proof}
Induct backwards on $\abs{B}$.
\begin{itemize}
\item
  Base case: $\abs{B} = n$, so $B = V$ \\
  $x_B = [T(B)]$ by first two cases of def \\
  RHS is the same: condition is always true, sum has 1 term, $\binom{n}{n} = 1$
\item
  Inductive step: $\abs{B} < n$, so $B \neq V$ \\
  IH holds for all $B'$ where $\abs{B'} = \abs{B}+1$ \\
  Case on $T(B)$
  \begin{itemize}
  \item
    If $\lnot T(B)$, then $x_B = 0$; WTS RHS $ = 0$ \\
    Given that $B = V_{\pi(:\abs{B})}$, if $k \geq \abs{B}$, then $B \subseteq V_{\pi(:k)}$,
    so $\lnot T(V_{\pi(:k)})$ \\
    Thus sum is $0$ for all relevant $\pi$, so expectation is $0$
  \item
    If $T(B)$, then consider $\Pi := \left\{\pi \in S_n \middle| B = V_{\pi(:\abs{B})}\right\}$ \\
    For all $j$ where $v_j \in V \setminus B$, define $B_j := B \cup \{v_j\}$ \\
    May partition $\Pi$ into $\Pi_j := \left\{\pi \in S_n \middle| B_j = V_{\pi(:\abs{B}+1)}\right\}$ \\
    All $\Pi_j$ are of equal size because this is equivalent to partitioning by $\pi(\abs{B}+1)$ \\
    IH holds for $B_j$, i.e.
    \begin{align*}
      x_{B_j}
      =\ &\E_{\pi \in S_n}\left(\sum_{k=\abs{B}+1}^n\binom{n}{k}\left[T\left(V_{\pi(:k)}\right)\right] \middle| B_j = V_{\pi(:\abs{B}+1)}\right) \\
      =\ &\E_{\pi \in \Pi_j}\left(\sum_{k=\abs{B}+1}^n\binom{n}{k}\left[T\left(V_{\pi(:k)}\right)\right]\right)
    \end{align*}
    Then
    \begin{align*}
      x_B
      =\ &\binom{n}{\abs{B}}+\E_{v_j \in V \setminus B}\left(x_{B_j}\right) \\
      =\ &\binom{n}{\abs{B}}+\E_{v_j \in V \setminus B}\left(\E_{\pi \in \Pi_j}\left(\sum_{k=\abs{B}+1}^n\binom{n}{k}\left[T\left(V_{\pi(:k)}\right)\right]\right)\right) \\
      =\ &\binom{n}{\abs{B}}+\E_{\pi \in \Pi}\left(\sum_{k=\abs{B}+1}^n\binom{n}{k}\left[T\left(V_{\pi(:k)}\right)\right]\right) \\
      =\ &\E_{\pi \in \Pi}\left(\binom{n}{\abs{B}}+\sum_{k=\abs{B}+1}^n\binom{n}{k}\left[T\left(V_{\pi(:k)}\right)\right]\right) \\
      =\ &\E_{\pi \in \Pi}\left(\sum_{k=\abs{B}}^n\binom{n}{k}\left[T\left(V_{\pi(:k)}\right)\right]\right) \\
      =\ &\E_{\pi \in S_n}\left(\sum_{k=\abs{B}}^n\binom{n}{k}\left[T\left(V_{\pi(:k)}\right)\right] \middle| B = V_{\pi(:\abs{B})}\right)
    \end{align*}
  \end{itemize}
\end{itemize}
\end{proof}
Finally, want to define the desired MC method and show it has the correct expectation \\
For $B \subseteq V$, define $C_B = \left\{v \in V \setminus B \middle| T(B \cup \{v\})\right\}$ \\
Define RVs $X_B$ by
\[
X_B :=
\begin{cases}
  0 & \text{if $\lnot T(B)$} \\
  1 & \text{if $T(B)$ and $B = V$} \\
  \binom{n}{\abs{B}}+\frac{\abs{C_B}}{\abs{V \setminus B}}X_{B \cup \{v\}} & \text{if $T(B)$ and $B \neq V$, for random $v \in C_B$}
\end{cases}
\]
\begin{lemma}
  For all $B \subseteq V$, $\E(X_B) = x_B$.
\end{lemma}
\begin{proof}
Induct backwards on $\abs{B}$.
\begin{itemize}
\item
  Base case: $\abs{B} = n$, so $B = V$ \\
  $\E(X_B) = [T(B)] = x_B$
\item
  Inductive step: $\abs{B} < n$, so $B \neq V$ \\
  IH holds for all $B'$ where $\abs{B'} = \abs{B}+1$ \\
  If $\lnot T(B)$, then $\E(X_B) = 0 = x_B$ \\
  If $T(B)$, then
  \begin{align*}
    &\E(X_B) \\
    =\ &\E_{v \in C_B}\left(\binom{n}{\abs{B}}+\frac{\abs{C_B}}{\abs{V \setminus B}}X_{B \cup \{v\}}\right) \\
    =\ &\binom{n}{\abs{B}}+\frac{\abs{C_B}}{\abs{V \setminus B}}\E_{v \in C_B}\left(X_{B \cup \{v\}}\right) \\
    =\ &\binom{n}{\abs{B}}+\frac{1}{\abs{V \setminus B}}\sum_{v \in C_B}\left(X_{B \cup \{v\}}\right) \\
    =\ &\binom{n}{\abs{B}}+\frac{1}{\abs{V \setminus B}}\sum_{v \in V \setminus B}\left(X_{B \cup \{v\}}\right) \\
    =\ &\binom{n}{\abs{B}}+\E_{v \in V \setminus B}\left(X_{B \cup \{v\}}\right) \\
    =\ &\binom{n}{\abs{B}}+\E_{v \in V \setminus B}\left(x_{B \cup \{v\}}\right) \\
    =\ &x_B
  \end{align*}
\end{itemize}
\end{proof}
\begin{theorem}
$\E(X_{\{\}}) = \abs{\left\{B \subseteq V \middle| T(B)\right\}}$.
\end{theorem}
\begin{proof}
  \begin{align*}
    \E(X_{\{\}})
    =\ &x_{\{\}} \\
    =\ &\E_{\pi \in S_n}\left(\sum_{k=\abs{\{\}}}^n\binom{n}{k}\left[T\left(V_{\pi(:k)}\right)\right] \middle| \{\} = V_{\pi(:\abs{\{\}})}\right) \\
    =\ &\E_{\pi \in S_n}\left(\sum_{k=0}^n\binom{n}{k}\left[T\left(V_{\pi(:k)}\right)\right]\right) \\
    =\ &\abs{\left\{B \subseteq V \middle| T(B)\right\}}
  \end{align*}
\end{proof}

\end{document}
