\documentclass{article}
\usepackage{amsmath}
\usepackage{amssymb}
\usepackage{amsthm}
\usepackage{graphicx}
\usepackage[margin=1in]{geometry}
\usepackage{hyperref}
\usepackage{caption}
\usepackage{float}
\graphicspath{{images/}}
\hypersetup{
  colorlinks=true,
  urlcolor=blue,
}
\begin{document}

\title{The Generalized Hockey-stick Identity}
\author{Aresh Pourkavoos}
\maketitle

\newtheorem*{GHSI}{Generalized Hockey-stick Identity}

\begin{GHSI}

For all $J, k_1, k_2 \in \mathbb{N}$,
\[\sum_{j_1+j_2=J}\binom{j_i+k_1}{j_1}\binom{j_2+k_2}{j_2} = \binom{J+k_1+k_2+1}{J}.\]

\end{GHSI}

\begin{proof}

Let $J, k_1, k_2 \in \mathbb{N}$. Define
\[f(j, k) = \binom{j+k}{k} =  \binom{j+k}{j} = \frac{(j+k)!}{j!k!}\]
so that the identity may be rewritten 
\[\sum_{j_1+j_2=J}f(j_1, k_1)f(j_2, k_2) = f(J, k_1+k_2+1).\]
Note $f(0, k)=f(j, 0)=1$ and $f(j+1, k+1)=f(j, k+1)+f(j+1, k)$ for all $j, k\in\mathbb{N}$.

Proof by induction over $J$ and $k_2$:
\begin{enumerate}
\item $J=0$ is trivial:
  \begin{align*}
    \sum_{j_1+j_2=0}f(j_1, k_1)f(j_2, k_2) &= f(0, k_1+k_2+1) \\
    f(0, k_1)f(0, k_2) &= f(0, k_1+k_2+1) \\
    1\times1 &= 1
  \end{align*}
\item $k_2=0$ reduces to the normal hockey stick identity:
  \begin{align*}
    \sum_{j_1+j_2=J}f(j_1, k_1)f(j_2, 0) &= f(J, k_1+0+1) \\
    \sum_{j_1=0}^{J}f(j_1, k_1) &= f(J, k_1+1)
  \end{align*}
\item $J=J'+1$, $k_2=k_2'+1$: Assume
  \begin{align*}
    \sum_{j_1+j_2=J'}f(j_1, k_1)f(j_2, k_2) = f(J', k_1+k_2+1), \\
    \sum_{j_1+j_2=J}f(j_1, k_1)f(j_2, k_2') = f(J, k_1+k_2'+1).
  \end{align*}
  Then
  \begin{align*}
    & \sum_{j_1+j_2=J}f(j_1, k_1)f(j_2, k_2) \\
    &= \sum_{j_1=0}^{J}f(j_1, k_1)f(J-j_1, k_2) \\
    &= \sum_{j_1=0}^{J'}f(j_1, k_1)f(J-j_1, k_2)+f(J, k_1) \\
    &= \sum_{j_1=0}^{J'}f(j_1, k_1)f(J'+1-j_1, k_2'+1)+f(J, k_1) \\
    &= \sum_{j_1=0}^{J'}f(j_1, k_1)(f(J'-j_1, k_2'+1)+f(J'+1-j_1, k_2'))+f(J, k_1) \\
    &= \sum_{j_1=0}^{J'}f(j_1, k_1)(f(J'-j_1, k_2)+f(J-j_1, k_2'))+f(J, k_1) \\
    &= \sum_{j_1=0}^{J'}(f(j_1, k_1)f(J'-j_1, k_2)+f(j_1, k_1)f(J-j_1, k_2'))+f(J, k_1) \\
    &= \sum_{j_1=0}^{J'}f(j_1, k_1)f(J'-j_1, k_2)+\sum_{j_1=0}^{J'}f(j_1, k_1)f(J-j_1, k_2')+f(J, k_1) \\
    &= \sum_{j_1=0}^{J'}f(j_1, k_1)f(J'-j_1, k_2)+\sum_{j_1=0}^{J}f(j_1, k_1)f(J-j_1, k_2') \\
    &= \sum_{j_1+j_2=J'}f(j_1, k_1)f(j_2, k_2)+\sum_{j_1+j_2=J}f(j_1, k_1)f(j_2, k_2') \\
    &= f(J', k_1+k_2+1)+f(J, k_1+k_2'+1) \\
    &= f(J, k_1+k_2+1). \\
  \end{align*}
\end{enumerate}

\end{proof}

\end{document}
